Charge!/src/LaterQuantTac.v
@@ -1,0 +1,29 @@
+Require Import Maps MapInterface MapFacts.
+Require Import ILogic Later BaseTactics ILQuantTac.
+
+Set Implicit Arguments.
+Unset Strict Implicit.
+
+Section PullForallLeft.
+
+	Context {A : Type} `{ILA : ILLater A}.
+
+	Definition later_op (p : find_res A) : find_res A :=
+		mkf (arrows_unop illater (find_closure p)).
+
+	Definition later_env_tac : env (find_res A) :=
+		env_add_unop (env_empty (find_res A)) 0 later_op.
+		
+	Lemma later_env_sound : env_sound_lr later_env later_env_tac find_res_eval_forall.
+	Proof.
+		unfold later_env_tac, later_env.
+		apply env_sound_lr_add_unop_tac. 
+		apply env_sound_lr_add_unop. apply env_sound_lr_empty. reflexivity.
+
+		exists illater. simpl. split. intuition.
+		split; [|apply _].
+		intros. destruct a.
+		simpl. induction find_types. simpl. reflexivity.
+		simpl in *. unfold find_res_eval_forall in *. simpl in *. setoid_rewrite IHfind_types.
+		apply spec_later_forall.
+	Qed.
